CMP rules; generalize CMP_eq versions to CMP_ZC

src/x86/instrrules.v
@@ -130,6 +130,36 @@ Definition specAtMemSpecDst dword ms (f: (DWORDorBYTE dword -> SPred) -> spec) :
           @ (regToAnyReg r ~= pbase)
     else f (fun v => offset :-> v) @ empSP.
 
+(*
+Definition lentails1 {T} (f g:T -> SPred):= forall x , f x |-- g x. 
+Definition lentails2 {T} (f g: (T -> SPred) -> spec) := forall x y, lentails1 x y -> 
+lentails (f x) (f y). 
+Global Instance specAtMemSpecDst_entails_m dword : 
+    Proper (eq --> lentails2 --> lentails) (@specAtMemSpecDst dword).
+Proof.
+  move => ms1 ms2 msE.
+  rewrite /Basics.flip in msE. subst. 
+  move => f1 f2 fE.
+  rewrite /Basics.flip/lentails2 in fE. 
+  rewrite /specAtMemSpecDst. 
+  destruct ms1. 
+  destruct sib.
+  destruct p.  
+  destruct o.  
+  destruct p. 
+  specintros => pbase1 ixval1.
+  rewrite /lentails1 in fE.
+  specsplit.
+  autorewrite with push_at. 
+  sbazooka. ssimpl.
+  simpl. specintros.  
+  autorewrite with push_at. specintros => pbase2 ixval2.
+  simpl. g fg.
+  move => P P' HP c _ <- Q Q' HQ. apply: basic_roc; try eassumption.
+    done.
+  Qed.
+*)
+
 Definition specAtMemSpec dword ms (f: DWORDorBYTE dword -> spec) :=
     let: mkMemSpec optSIB offset := ms in
     if optSIB is Some(r, ixspec)
@@ -958,7 +988,7 @@ Proof.
 Qed. 
 
 (*---------------------------------------------------------------------------
-    ADD instruction
+    ADD and SUB instructions
   ---------------------------------------------------------------------------*)
 (* Generic ADD/SUB rule *)
 Lemma ADDSUB_rule isSUB d (ds:DstSrc d) v1 :
@@ -1143,6 +1173,7 @@ Ltac basicADDSUB :=
   | _ => idtac
   end.
 
+(* Special cases *)
 (* ADD r, v2 *)
 Corollary ADD_RI_rule (r:Reg) v1 (v2:DWORD):
   |-- basic (r~=v1 ** OSZCP_Any) (ADD r, v2)
@@ -1181,6 +1212,398 @@ Corollary ADD_RM_rule (pd:BITS 32) (r1 r2:Reg) v1 (v2:DWORD) (offset:nat):
              OSZCP (computeOverflow v1 v2 v) (msb v) (v == #0) carry (lsb v)).
 Proof. basicADDSUB. elim: (adcB _) => [carry v]. by ssimpl. Qed.   
 
+Corollary ADD_RM_ruleNoFlags (pd:BITS 32) (r1 r2:Reg) v1 (v2:DWORD) (offset:nat):
+  |-- basic (r1~=v1) (ADD r1, [r2 + offset]) (r1~=addB v1 v2)
+             @ (r2 ~= pd ** pd +# offset :-> v2 ** OSZCP_Any).
+Proof.
+autorewrite with push_at.
+basicADDSUB.  
+rewrite /OSZCP/OSZCP_Any/stateIsAny/addB/dropmsb/snd.
+elim: (adcB _) => [carry v].
+sbazooka.
+Qed.   
+
+Lemma SUB_RM_rule (pd:BITS 32) (r1 r2:Reg) v1 (v2:DWORD) (offset:nat):
+  |-- basic (r1~=v1 ** r2 ~= pd ** pd +# offset :-> v2 ** OSZCP_Any)
+            (SUB r1, [r2 + offset])
+            (let: (carry,v) := sbbB false v1 v2 in
+             r1~=v ** r2 ~= pd ** pd +# offset :-> v2 **
+             OSZCP (computeOverflow v1 v2 v) (msb v) (v == #0) carry (lsb v)).
+Proof. basicADDSUB. elim (sbbB _) => [carry v]. by ssimpl. Qed.
+
+Corollary SUB_RM_ruleNoFlags (pd:BITS 32) (r1 r2:Reg) v1 (v2:DWORD) (offset:nat):
+  |-- basic (r1~=v1) (SUB r1, [r2 + offset]) (r1~=subB v1 v2)
+             @ (r2 ~= pd ** pd +# offset :-> v2 ** OSZCP_Any).
+Proof.
+autorewrite with push_at. rewrite /subB. 
+elim E: (sbbB _ _ _) => [carry v].
+basicADDSUB. 
+rewrite /OSZCP/OSZCP_Any/stateIsAny/snd E. sbazooka.
+Qed.   
+
+Lemma SUB_RR_rule (r1 r2:Reg) v1 (v2:DWORD):
+  |-- basic (r1~=v1 ** r2~=v2 ** OSZCP_Any) (SUB r1, r2)
+            (let: (carry,v) := sbbB false v1 v2 in r1~=v  ** r2~=v2 **
+             OSZCP (computeOverflow v1 v2 v) (msb v) (v == #0) carry (lsb v)).
+Proof. basicADDSUB. elim (sbbB _ _ _) => [carry v]. by ssimpl. Qed. 
+
+Lemma SUB_RI_rule (r1:Reg) v1 (v2:DWORD):
+  |-- basic (r1~=v1 ** OSZCP_Any) (SUB r1, v2)
+            (let: (carry,v) := sbbB false v1 v2 in 
+             r1~=v ** OSZCP (computeOverflow v1 v2 v) (msb v) (v == #0) carry (lsb v)).
+Proof. basicADDSUB. Qed. 
+
+(*---------------------------------------------------------------------------
+    CMP instruction
+  ---------------------------------------------------------------------------*)
+
+(* Generic rule *)
+Lemma CMP_rule d (ds:DstSrc d) v1 :
+   |-- specAtDstSrc ds (fun D v2 =>
+       basic (D v1 ** OSZCP_Any)
+             (BOP d OP_CMP ds)
+             (let: (carry,v) := sbbB false v1 v2 in
+              D v1 ** OSZCP (computeOverflow v1 v2 v) (msb v) (v == #0) carry (lsb v))).
+Proof.
+  rewrite /specAtDstSrc. 
+  destruct ds. 
+  (* RR *)
+  specintros => v2. 
+  autorewrite with push_at. apply TRIPLE_basic => R. rewrite /evalInstr/evalDstSrc/evalDstR.
+  triple_apply evalDWORDorBYTEReg_rule. 
+  triple_apply evalDWORDorBYTEReg_rule. 
+  rewrite /evalBinOp/evalArithOpNoCarry.
+  triple_apply triple_pre_introFlags => o s z c pf. rewrite /OSZCP.
+  elim: (_ false v1 v2) => [carry v].
+  triple_apply triple_doSetFlagSep.
+  triple_apply triple_doSetFlagSep.
+  triple_apply triple_doUpdateZPS. triple_apply triple_skip. 
+  (* RM *)
+  rewrite /specAtMemSpec. 
+  elim:src => [optSIB offset].
+  elim: optSIB => [[base ixopt] |].
+  case: ixopt => [[ixr sc] |]. 
+(* Indexed *)
+  + specintros => v2 pbase ixval. 
+    autorewrite with push_at. apply TRIPLE_basic => R. rewrite /evalInstr/evalDstSrc/evalDstR.
+    triple_apply evalDWORDorBYTEReg_rule. 
+    triple_apply evalMemSpec_rule. 
+    triple_apply triple_letGetDWORDorBYTESep. 
+    rewrite /evalBinOp/evalArithOpNoCarry.
+    triple_apply triple_pre_introFlags => o s z c pf. rewrite /OSZCP.
+    (elim: (_ false v1 v2) => [carry v];
+    triple_apply triple_doSetFlagSep;
+    triple_apply triple_doSetFlagSep; 
+    triple_apply triple_doUpdateZPS; 
+    triple_apply triple_skip). 
+(* Non-indexed *)
+  + specintros => v2 pbase. 
+    autorewrite with push_at. apply TRIPLE_basic => R. rewrite /evalInstr/evalDstSrc/evalDstR.
+    triple_apply evalDWORDorBYTEReg_rule.
+    triple_apply evalMemSpecNone_rule.    
+    triple_apply triple_pre_introFlags => o s z c pf. rewrite /OSZCP.
+    triple_apply triple_letGetDWORDorBYTESep. 
+    rewrite /evalBinOp/evalArithOpNoCarry.
+    (elim: (_ false v1 v2) => [carry v];
+    triple_apply triple_doSetFlagSep;
+    triple_apply triple_doSetFlagSep; 
+    triple_apply triple_doUpdateZPS; 
+    triple_apply triple_skip). 
+(* offset only *)
+  + specintro => v2. 
+    autorewrite with push_at. apply TRIPLE_basic => R. rewrite /evalInstr/evalDstSrc/evalDstR.
+    triple_apply evalDWORDorBYTEReg_rule.  rewrite /evalMemSpec.
+    triple_apply triple_letGetDWORDorBYTESep. 
+    triple_apply triple_pre_introFlags => o s z c pf. rewrite /OSZCP.
+    rewrite /evalBinOp/evalArithOpNoCarry.
+    (elim: (_ false v1 v2) => [carry v];
+    triple_apply triple_doSetFlagSep;
+    triple_apply triple_doSetFlagSep; 
+    triple_apply triple_doUpdateZPS; 
+    triple_apply triple_skip). 
+
+  (* MR *)
+  specintros => v2. rewrite /specAtMemSpecDst. 
+  elim:dst => [optSIB offset].
+  case: optSIB => [[base ixopt] |].  
+  case: ixopt => [[ixr sc] |]. 
+(* Indexed *)
+  + specintros => pbase ixval. autorewrite with push_at. apply TRIPLE_basic => R. 
+    rewrite /evalInstr/evalDstSrc/evalDstM. 
+    triple_apply evalMemSpec_rule. 
+    triple_apply triple_letGetDWORDorBYTESep. 
+    triple_apply evalDWORDorBYTEReg_rule.
+    triple_apply triple_pre_introFlags => o s z c pf. rewrite /OSZCP.
+    rewrite /evalBinOp/evalArithOpNoCarry.
+    (elim: (_ false v1 v2) => [carry v];
+    triple_apply triple_doSetFlagSep;
+    triple_apply triple_doSetFlagSep;
+    triple_apply triple_doUpdateZPS;
+    triple_apply triple_skip). 
+(* Non-indexed *)
+  + specintros => pbase. autorewrite with push_at. apply TRIPLE_basic => R. 
+    rewrite /evalInstr/evalDstSrc/evalDstM. 
+    triple_apply evalMemSpecNone_rule.
+    triple_apply triple_letGetDWORDorBYTESep. 
+    triple_apply evalDWORDorBYTEReg_rule. 
+    triple_apply triple_pre_introFlags => o s z c pf. rewrite /OSZCP.
+    rewrite /evalBinOp/evalArithOpNoCarry.
+    (elim: (_ false v1 v2) => [carry v];
+    triple_apply triple_doSetFlagSep;
+    triple_apply triple_doSetFlagSep;
+    triple_apply triple_doUpdateZPS;
+    triple_apply triple_skip). 
+(* Offset only *)
+  + autorewrite with push_at. apply TRIPLE_basic => R. 
+    rewrite /evalInstr/evalDstSrc/evalDstM/evalMemSpec.
+    triple_apply triple_letGetDWORDorBYTESep. 
+    triple_apply evalDWORDorBYTEReg_rule. 
+    triple_apply triple_pre_introFlags => o s z c pf. rewrite /OSZCP.
+    rewrite /evalBinOp/evalArithOpNoCarry.
+    (elim: (_ false v1 v2) => [carry v];
+    triple_apply triple_doSetFlagSep;
+    triple_apply triple_doSetFlagSep;
+    triple_apply triple_doUpdateZPS;
+    triple_apply triple_skip). 
+  (* RI *)
+  apply TRIPLE_basic => R.
+  rewrite /evalInstr/evalDstSrc/evalDstR. 
+  triple_apply evalDWORDorBYTEReg_rule. 
+  triple_apply triple_pre_introFlags => o sf zf cf pf. rewrite /OSZCP.
+    rewrite /evalBinOp/evalArithOpNoCarry.
+    (elim: (_ false _ _) => [carry v];
+    triple_apply triple_doSetFlagSep;
+    triple_apply triple_doSetFlagSep;
+    triple_apply triple_doUpdateZPS;
+    triple_apply triple_skip). 
+
+  (* MI *)
+  rewrite /specAtMemSpecDst. 
+  elim:dst => [optSIB offset].
+  elim:optSIB => [[base ixopt] |].
+  case: ixopt => [[ixr sc] |]. 
+
+(* Indexed *)
+  + specintros => pbase ixval. autorewrite with push_at. apply TRIPLE_basic => R. 
+    rewrite /evalInstr/evalDstSrc/evalDstM.
+    triple_apply evalMemSpec_rule. 
+    triple_apply triple_letGetDWORDorBYTESep.    
+    triple_apply triple_pre_introFlags => o s z cf pf. rewrite /OSZCP.
+    rewrite /evalBinOp/evalArithOpNoCarry.
+    (elim: (_ false _ _) => [carry v];
+    triple_apply triple_doSetFlagSep;
+    triple_apply triple_doSetFlagSep;
+    triple_apply triple_doUpdateZPS;
+    triple_apply triple_skip). 
+(* Non-indexed *)
+  + specintros => pbase. autorewrite with push_at. apply TRIPLE_basic => R. 
+    repeat (autounfold with eval). rewrite /evalDstSrc/evalDstM. 
+    triple_apply evalMemSpecNone_rule. 
+    triple_apply triple_letGetDWORDorBYTESep. 
+    triple_apply triple_pre_introFlags => o s z cf pf. rewrite /OSZCP.
+    rewrite /evalBinOp/evalArithOpNoCarry.
+    (elim: (_ false _ _) => [carry v];
+    triple_apply triple_doSetFlagSep;
+    triple_apply triple_doSetFlagSep;
+    triple_apply triple_doUpdateZPS;
+    triple_apply triple_skip). 
+(* Offset only *)
+  + autorewrite with push_at. apply TRIPLE_basic => R. 
+    rewrite /evalInstr/evalDstSrc/evalDstM/evalMemSpec. 
+    triple_apply triple_letGetDWORDorBYTESep. 
+    triple_apply triple_pre_introFlags => o s z cf pf. rewrite /OSZCP.
+    rewrite /evalBinOp/evalArithOpNoCarry.
+    (elim: (_ false _ _) => [carry v];
+    triple_apply triple_doSetFlagSep;
+    triple_apply triple_doSetFlagSep;
+    triple_apply triple_doUpdateZPS;
+    triple_apply triple_skip). 
+Qed.   
+
+Lemma sbbB_ZC n (r : BITS n) carry (v1 v: BITS n) :
+  sbbB false v1 v = (carry, r) ->
+   ZF~=(r == #(0)) ** CF~=carry |-- CF~=ltB v1 v ** ZF~=(v1 == v).
+Proof. move => E. 
+  have S0 := subB_eq0 v1 v. rewrite /subB E/snd in S0. rewrite S0.
+  have HH := (sbbB_ltB_leB v1 v). rewrite E/fst in HH. 
+  destruct carry. + rewrite HH. by ssimpl. + rewrite ltBNle HH /negb. by ssimpl.
+Qed.
+
+(* Generic rule with C and Z flags determining ltB and equality respectively *)
+Lemma CMP_ruleZC d (ds:DstSrc d) v1 :
+   |-- specAtDstSrc ds (fun D v2 =>
+       basic (D v1 ** OSZCP_Any)
+             (BOP d OP_CMP ds)
+             (D v1 ** OF? ** SF? ** PF? ** CF ~= ltB v1 v2 ** ZF ~= (v1==v2))).
+Proof. 
+have C := (CMP_rule ds) v1. rewrite /specAtDstSrc in C. rewrite /specAtDstSrc. 
+destruct ds. 
++ specintros => v. autorewrite with push_at. 
+  eapply basic_basic. eforalls C. autorewrite with push_at in C. 
+  apply C. sbazooka. elim E:(sbbB false v1 v) => [carry r].
+  rewrite /OSZCP/stateIsAny. sbazooka. 
+  by apply sbbB_ZC.   
++ destruct src as [optSIB offset].
+  destruct optSIB as [[base ixopt] |].  
+  destruct ixopt as [[ixr sc] |]. 
+  rewrite /specAtMemSpec. rewrite /specAtMemSpec in C. 
+  specintros => v pbase ixval. autorewrite with push_at. 
+  eapply basic_basic. eforalls C. autorewrite with push_at in C.
+  apply C. sbazooka. elim E:(sbbB false v1 v) => [carry r].
+  rewrite /OSZCP/stateIsAny. sbazooka. 
+  by apply sbbB_ZC.   
+  rewrite /specAtMemSpec. rewrite /specAtMemSpec in C. 
+  specintros => v pbase. autorewrite with push_at. 
+  eapply basic_basic. eforalls C. autorewrite with push_at in C.
+  apply C. sbazooka. elim E:(sbbB false v1 v) => [carry r].
+  rewrite /OSZCP/stateIsAny. sbazooka. 
+  by apply sbbB_ZC.   
+  rewrite /specAtMemSpec. rewrite /specAtMemSpec in C. 
+  specintros => v. autorewrite with push_at. 
+  eapply basic_basic. eforalls C. autorewrite with push_at in C.
+  apply C. sbazooka. elim E:(sbbB false v1 v) => [carry r].
+  rewrite /OSZCP/stateIsAny. sbazooka. 
+  by apply sbbB_ZC.   
+  specintros => v. rewrite /specAtMemSpecDst. rewrite /specAtMemSpecDst in C. 
+  destruct dst as [optSIB offset]. 
+  destruct optSIB as [[base ixopt] |]. 
+  destruct ixopt as [[ixr sc] |]. 
+  specintros => pbase ixval. autorewrite with push_at.
+  eapply basic_basic. eforalls C. autorewrite with push_at in C.
+  apply C. sbazooka. elim E:(sbbB false v1 v) => [carry r].
+  rewrite /OSZCP/stateIsAny. sbazooka. 
+  by apply sbbB_ZC.   
+  specintros => pbase. autorewrite with push_at.
+  eapply basic_basic. eforalls C. autorewrite with push_at in C.
+  apply C. sbazooka. elim E:(sbbB false v1 v) => [carry r].
+  rewrite /OSZCP/stateIsAny. sbazooka. 
+  by apply sbbB_ZC.   
+autorewrite with push_at.
+  eapply basic_basic. eforalls C. autorewrite with push_at in C.
+  apply C. sbazooka. elim E:(sbbB false v1 v) => [carry r].
+  rewrite /OSZCP/stateIsAny. sbazooka. 
+  by apply sbbB_ZC.   
+
+  eapply basic_basic. eforalls C. autorewrite with push_at in C.
+  apply C. sbazooka. elim E:(sbbB false v1 c) => [carry r].
+  rewrite /OSZCP/stateIsAny. sbazooka. 
+  by apply sbbB_ZC.   
+
+rewrite /specAtMemSpecDst. rewrite /specAtMemSpecDst in C. 
+  destruct dst as [optSIB offset]. 
+  destruct optSIB as [[base ixopt] |]. 
+  destruct ixopt as [[ixr sc] |]. 
+  specintros => pbase ixval. autorewrite with push_at.
+  eapply basic_basic. eforalls C. autorewrite with push_at in C.
+  apply C. sbazooka. elim E:(sbbB false v1 c) => [carry r].
+  rewrite /OSZCP/stateIsAny. sbazooka. 
+  by apply sbbB_ZC.   
+  specintros => pbase. autorewrite with push_at.
+  eapply basic_basic. eforalls C. autorewrite with push_at in C.
+  apply C. sbazooka. elim E:(sbbB false v1 c) => [carry r].
+  rewrite /OSZCP/stateIsAny. sbazooka. 
+  by apply sbbB_ZC.   
+autorewrite with push_at.
+  eapply basic_basic. eforalls C. autorewrite with push_at in C.
+  apply C. sbazooka. elim E:(sbbB false v1 c) => [carry r].
+  rewrite /OSZCP/stateIsAny. sbazooka. 
+  by apply sbbB_ZC.   
+Qed.   
+
+Ltac basicCMP :=
+  try unfold makeBOP;
+  match goal with
+  | |- |-- basic ?p (@BOP ?d OP_CMP ?a) ?q => basicapply (@CMP_rule d a)  
+  | _ => idtac
+  end.
+
+Ltac basicCMP_ZC :=
+  try unfold makeBOP;
+  match goal with
+  | |- |-- basic ?p (@BOP ?d OP_CMP ?a) ?q => basicapply (@CMP_ruleZC d a)  
+  | _ => idtac
+  end.
+
+
+(* Special cases *)
+Lemma CMP_RI_rule (r1:Reg) v1 (v2:DWORD):
+  |-- basic (r1 ~= v1 ** OSZCP_Any) (CMP r1, v2)
+            (let: (carry,res) := sbbB false v1 v2 in
+             r1 ~= v1 ** OSZCP (computeOverflow v1 v2 res) (msb res)
+                         (res == #0) carry (lsb res)).
+Proof. basicCMP. Qed.
+
+Lemma CMP_RbI_rule (r1:BYTEReg) (v1 v2:BYTE):
+  |-- basic (BYTEregIs r1 v1 ** OSZCP_Any) (BOP false OP_CMP (DstSrcRI false r1 v2))
+            (let: (carry,res) := sbbB false v1 v2 in
+  BYTEregIs r1 v1 ** OSZCP (computeOverflow v1 v2 res) (msb res) (res == #0) carry (lsb res)).
+Proof. basicCMP. Qed.
+
+Lemma CMP_RM_rule (pd:BITS 32) (r1 r2:Reg) offset (v1 v2:DWORD) :
+  |-- basic (r1 ~= v1 ** r2 ~= pd ** pd +# offset :-> v2 ** OSZCP_Any)
+            (CMP r1, [r2+offset])
+            (let (carry,res) := sbbB false v1 v2 in
+             r1 ~= v1 ** r2 ~= pd ** pd +# offset :-> v2 **
+             OSZCP (computeOverflow v1 v2 res) (msb res)
+                   (res == #0) carry (lsb res)).
+Proof. basicCMP. 
+case E: (sbbB false v1 v2) => [carry res]. 
+sbazooka. 
+Qed. 
+
+Lemma CMP_MR_rule (pd:BITS 32) (r1 r2:Reg) offset (v1 v2:DWORD):
+  |-- basic (r1 ~= v1 ** r2 ~= pd ** pd +# offset :-> v2 ** OSZCP_Any)
+            (CMP [r2+offset], r1)
+            (let (carry,res) := sbbB false v2 v1 in
+             r1 ~= v1 ** r2 ~= pd ** pd +# offset :-> v2 **
+             OSZCP (computeOverflow v2 v1 res) (msb res)
+                   (res == #0) carry (lsb res)).
+Proof. basicCMP.
+case E: (sbbB false v2 v1) => [carry res]. 
+sbazooka. 
+Qed. 
+
+
+Lemma CMP_RR_rule (r1 r2:Reg) v1 (v2:DWORD):
+  |-- basic (r1 ~= v1 ** r2 ~= v2 ** OSZCP_Any) (CMP r1, r2)
+            (let: (carry,res) := sbbB false v1 v2 in
+             r1 ~= v1 ** r2 ~= v2 **
+              OSZCP (computeOverflow v1 v2 res) (msb res)
+                    (res == #0) carry (lsb res)).
+Proof. basicCMP. destruct (sbbB false v1 v2); by ssimpl. Qed. 
+
+
+Lemma CMP_RI_ZC_rule (r1:Reg) v1 (v2:DWORD):
+  |-- basic (r1 ~= v1 ** OSZCP_Any) (CMP r1, v2)
+            (r1 ~= v1 ** OF? ** SF? ** PF? ** CF ~= ltB v1 v2 ** ZF ~= (v1==v2)).
+Proof. basicCMP_ZC. Qed. 
+
+Lemma CMP_MbR_ZC_rule (r1:Reg) (r2: BYTEReg) (p:DWORD) (v1 v2:BYTE):
+  |-- basic (r1 ~= p ** BYTEregIs r2 v2 ** p :-> v1 ** OSZCP_Any) (CMP [r1], r2)
+            (r1 ~= p ** BYTEregIs r2 v2 ** p :-> v1 ** OF? ** SF? ** PF? ** 
+                        CF ~= ltB v1 v2 ** ZF ~= (v1==v2)).
+Proof. basicCMP_ZC. Qed. 
+
+Lemma CMP_MbI_ZC_rule (r1:Reg) (p:DWORD) (v1 v2:BYTE):
+  |-- basic (r1 ~= p ** p :-> v1 ** OSZCP_Any) (CMP BYTE [r1], v2)
+            (r1 ~= p ** p :-> v1 ** OF? ** SF? ** PF? ** 
+                         CF ~= ltB v1 v2 ** ZF ~= (v1==v2)).
+Proof. basicCMP_ZC. Qed. 
+
+Lemma CMP_MbxI_ZC_rule (r1:Reg) (r2:NonSPReg) (p ix:DWORD) (v1 v2:BYTE):
+  |-- basic (r1 ~= p ** r2 ~= ix ** addB p ix :-> v1 ** OSZCP_Any) (CMP BYTE [r1 + r2 + 0], v2)
+            (r1 ~= p ** r2 ~= ix ** addB p ix :-> v1 ** OF? ** SF? ** PF? ** 
+                         CF ~= ltB v1 v2 ** ZF ~= (v1==v2)).
+Proof. basicCMP_ZC; rewrite /scaleBy; by ssimpl. Qed. 
+
+
+Lemma CMP_RbI_ZC_rule (r1:BYTEReg) (v1 v2:BYTE):
+  |-- basic (BYTEregIs r1 v1 ** OSZCP_Any) (BOP false OP_CMP (DstSrcRI false r1 v2))
+            (BYTEregIs r1 v1 ** OF? ** SF? ** PF? ** 
+                         CF ~= ltB v1 v2 ** ZF ~= (v1==v2)).
+Proof. basicCMP_ZC. Qed.
+
+
 Lemma XOR_RR_rule (r1 r2:Reg) v1 (v2:DWORD):
   |-- basic (r1~=v1 ** r2~=v2 ** OSZCP_Any) (XOR r1, r2)
             (r1~=xorB v1 v2 ** r2~=v2 ** OSZCP false (msb (xorB v1 v2))
@@ -1196,14 +1619,6 @@ Proof.
   triple_apply triple_doUpdateZPS. 
   triple_apply triple_setRegSep. 
 Qed. 
-
-Lemma SUB_RM_rule (pd:BITS 32) (r1 r2:Reg) v1 (v2:DWORD) (offset:nat):
-  |-- basic (r1~=v1 ** r2 ~= pd ** pd +# offset :-> v2 ** OSZCP_Any)
-            (SUB r1, [r2 + offset])
-            (let: (carry,v) := sbbB false v1 v2 in
-             r1~=v ** r2 ~= pd ** pd +# offset :-> v2 **
-             OSZCP (computeOverflow v1 v2 v) (msb v) (v == #0) carry (lsb v)).
-Proof. basicADDSUB. elim (sbbB _) => [carry v]. by ssimpl. Qed.
 
 Lemma ADC_RI_rule (r1:Reg) v1 (v2:DWORD) carry v o s z c p:
   adcB c v1 v2 = (carry,v) ->
@@ -1223,28 +1638,6 @@ Proof.
   triple_apply triple_doUpdateZPS. 
   triple_apply triple_setRegSep. 
 Qed. 
-
-Corollary ADD_RM_ruleNoFlags (pd:BITS 32) (r1 r2:Reg) v1 (v2:DWORD) (offset:nat):
-  |-- basic (r1~=v1) (ADD r1, [r2 + offset]) (r1~=addB v1 v2)
-             @ (r2 ~= pd ** pd +# offset :-> v2 ** OSZCP_Any).
-Proof.
-autorewrite with push_at.
-basicADDSUB.  
-rewrite /OSZCP/OSZCP_Any/stateIsAny/addB/dropmsb/snd.
-elim: (adcB _) => [carry v].
-sbazooka.
-Qed.   
-
-Corollary SUB_RM_ruleNoFlags (pd:BITS 32) (r1 r2:Reg) v1 (v2:DWORD) (offset:nat):
-  |-- basic (r1~=v1) (SUB r1, [r2 + offset]) (r1~=subB v1 v2)
-             @ (r2 ~= pd ** pd +# offset :-> v2 ** OSZCP_Any).
-Proof.
-autorewrite with push_at. rewrite /subB. 
-elim E: (sbbB _ _ _) => [carry v].
-basicADDSUB. 
-rewrite /OSZCP/OSZCP_Any/stateIsAny/snd E. sbazooka.
-Qed.   
-
 
 (*---------------------------------------------------------------------------
     AND instruction
@@ -1490,221 +1883,6 @@ basicapply (@XOR_RM_rule pd r1 r2 v1 v2 offset (xorB v1 v2) (refl_equal _)).
 rewrite /OSZCP/OSZCP_Any/stateIsAny/snd. sbazooka. 
 Qed.   
 
-
-Lemma SUB_RR_rule (r1 r2:Reg) v1 (v2:DWORD):
-  |-- basic (r1~=v1 ** r2~=v2 ** OSZCP_Any) (SUB r1, r2)
-            (let: (carry,v) := sbbB false v1 v2 in r1~=v  ** r2~=v2 **
-             OSZCP (computeOverflow v1 v2 v) (msb v) (v == #0) carry (lsb v)).
-Proof. basicADDSUB. elim (sbbB _ _ _) => [carry v]. by ssimpl. Qed. 
-
-Lemma SUB_RI_rule (r1:Reg) v1 (v2:DWORD):
-  |-- basic (r1~=v1 ** OSZCP_Any) (SUB r1, v2)
-            (let: (carry,v) := sbbB false v1 v2 in 
-             r1~=v ** OSZCP (computeOverflow v1 v2 v) (msb v) (v == #0) carry (lsb v)).
-Proof. basicADDSUB. Qed. 
-
-Lemma CMP_RI_rule (r1:Reg) v1 (v2:DWORD) carry res:
-  sbbB false v1 v2 = (carry, res) ->
-  |-- basic (r1 ~= v1 ** OSZCP_Any) (CMP r1, v2)
-            (r1 ~= v1 ** OSZCP (computeOverflow v1 v2 res) (msb res)
-                         (res == #0) carry (lsb res)).
-Proof.
-  move => E. apply TRIPLE_basic => R.
-  repeat autounfold with eval.  
-  rewrite /evalDstSrc/evalDstR.
-  triple_apply evalReg_rule. 
-  rewrite E.
-  triple_apply triple_pre_introFlags => o s z c p. rewrite /OSZCP.
-  triple_apply triple_doSetFlagSep. 
-  triple_apply triple_doSetFlagSep. 
-  triple_apply triple_doUpdateZPS. 
-  triple_apply triple_skip. 
-Qed. 
-
-Lemma CMP_RbI_rule (r1:BYTEReg) (v1 v2:BYTE) carry res:
-  sbbB false v1 v2 = (carry, res) ->
-  |-- basic (BYTEregIs r1 v1 ** OSZCP_Any) (BOP false OP_CMP (DstSrcRI false r1 v2))
-            (BYTEregIs r1 v1 ** OSZCP (computeOverflow v1 v2 res) (msb res) (res == #0) carry (lsb res)).
-Proof.
-  move => E. apply TRIPLE_basic => R.
-  repeat autounfold with eval.  
-  rewrite /evalDstSrc/evalDstR.
-  triple_apply evalBYTEReg_rule.
-  rewrite E.
-  triple_apply triple_pre_introFlags => o s z c p. rewrite /OSZCP.
-  triple_apply triple_doSetFlagSep. 
-  triple_apply triple_doSetFlagSep. 
-  triple_apply triple_doUpdateZPS. 
-  triple_apply triple_skip. 
-Qed. 
-
-Lemma CMP_RI_eq_rule (r1:Reg) v1 (v2:DWORD):
-  |-- basic (r1 ~= v1 ** OSZCP_Any) (CMP r1, v2)
-            (r1 ~= v1 ** OF? ** SF? ** CF? ** PF? ** 
-                         ZF ~= (v1==v2)).
-Proof.
-case E: (sbbB false v1 v2) => [carry res]. 
-eapply basic_basic.
-apply (CMP_RI_rule E).
-by ssimpl.  
-rewrite /OSZCP/stateIsAny. sbazooka. 
-have: res = subB v1 v2. 
-rewrite /subB. by rewrite E.  
-move ->.
-by rewrite subB_eq0. 
-Qed. 
-
-Lemma CMP_MbR_eq_rule (r1:Reg) (r2: BYTEReg) (p:DWORD) (v1 v2:BYTE):
-  |-- basic (r1 ~= p ** BYTEregIs r2 v2 ** p :-> v1 ** OSZCP_Any) (CMP [r1], r2)
-            (r1 ~= p ** BYTEregIs r2 v2 ** p :-> v1 ** OF? ** SF? ** CF? ** PF? ** 
-                         ZF ~= (v1==v2)).
-Proof.
-  apply TRIPLE_basic => R.
-  repeat autounfold with eval.  
-  rewrite /evalDstSrc/evalDstR/evalDstM.
-  triple_apply evalMemSpecNone_rule.
-  rewrite addB0/scaleBy.
-  triple_apply triple_letGetBYTESep. 
-  triple_apply triple_pre_introFlags => o s z c pf. rewrite /OSZCP.
-  triple_apply evalBYTEReg_rule. 
-case E: (sbbB false v1 v2) => [carry res].   
-  triple_apply triple_doSetFlagSep. 
-  triple_apply triple_doSetFlagSep. 
-  triple_apply triple_doUpdateZPS. 
-  triple_apply triple_skip. rewrite /stateIsAny.
-  sbazooka. 
-  have H:= (subB_eq0 v1 v2). rewrite /subB in H.
-  rewrite E in H. by rewrite H. 
-Qed. 
-
-Lemma CMP_MbI_eq_rule (r1:Reg) (p:DWORD) (v1 v2:BYTE):
-  |-- basic (r1 ~= p ** p :-> v1 ** OSZCP_Any) (CMP BYTE [r1], v2)
-            (r1 ~= p ** p :-> v1 ** OF? ** SF? ** CF? ** PF? ** 
-                         ZF ~= (v1==v2)).
-Proof.
-  apply TRIPLE_basic => R.
-  repeat autounfold with eval.  
-  rewrite /evalDstSrc/evalDstR/evalDstM.
-  triple_apply evalMemSpecNone_rule.
-  rewrite addB0/scaleBy.
-  triple_apply triple_letGetBYTESep. 
-case E: (sbbB false v1 v2) => [carry res].   
-  triple_apply triple_pre_introFlags => o s z c pf. rewrite /OSZCP.
-  triple_apply triple_doSetFlagSep. 
-  triple_apply triple_doSetFlagSep. 
-  triple_apply triple_doUpdateZPS. 
-  triple_apply triple_skip. rewrite /stateIsAny.
-  sbazooka. 
-  have H:= (subB_eq0 v1 v2). rewrite /subB in H.
-  rewrite E in H. by rewrite H.
-Qed. 
-
-
-Lemma CMP_MbxI_eq_rule (r1:Reg) (r2:NonSPReg) (p ix:DWORD) (v1 v2:BYTE):
-  |-- basic (r1 ~= p ** r2 ~= ix ** addB p ix :-> v1 ** OSZCP_Any) (CMP BYTE [r1 + r2 + 0], v2)
-            (r1 ~= p ** r2 ~= ix ** addB p ix :-> v1 ** OF? ** SF? ** CF? ** PF? ** 
-                         ZF ~= (v1==v2)).
-Proof.
-  apply TRIPLE_basic => R.
-  repeat autounfold with eval.  
-  rewrite /evalDstSrc/evalDstR/evalDstM.
-  triple_apply evalMemSpec_rule.
-  rewrite addB0/scaleBy.
-  triple_apply triple_letGetBYTESep. 
-case E: (sbbB false v1 v2) => [carry res].   
-  triple_apply triple_pre_introFlags => o s z c pf. rewrite /OSZCP.
-  triple_apply triple_doSetFlagSep. 
-  triple_apply triple_doSetFlagSep. 
-  triple_apply triple_doUpdateZPS. 
-  triple_apply triple_skip.
-  rewrite /stateIsAny.  sbazooka. 
-  have H:= (subB_eq0 v1 v2). rewrite /subB in H.
-  rewrite E in H. by rewrite H. 
-Qed. 
-
-
-Lemma CMP_RbI_eq_rule (r1:BYTEReg) (v1 v2:BYTE):
-  |-- basic (BYTEregIs r1 v1 ** OSZCP_Any) (BOP false OP_CMP (DstSrcRI false r1 v2))
-            (BYTEregIs r1 v1 ** OF? ** SF? ** CF? ** PF? ** 
-                         ZF ~= (v1==v2)).
-Proof.
-  apply TRIPLE_basic => R.
-  repeat autounfold with eval.  
-  rewrite /evalDstSrc/evalDstR/evalDstM.
-  triple_apply evalBYTEReg_rule.
-case E: (sbbB false v1 v2) => [carry res].   
-  triple_apply triple_pre_introFlags => o s z c pf. rewrite /OSZCP.
-  triple_apply triple_doSetFlagSep. 
-  triple_apply triple_doSetFlagSep. 
-  triple_apply triple_doUpdateZPS. 
-  triple_apply triple_skip.
-  rewrite /stateIsAny. sbazooka. 
-  have H:= (subB_eq0 v1 v2). rewrite /subB in H. rewrite E in H. 
-  by rewrite H. 
-Qed. 
-
-
-Lemma CMP_RM_rule (pd:BITS 32) (r1 r2:Reg) offset (v1 v2:DWORD) carry res :
-  sbbB false v1 v2 = (carry, res) ->
-  |-- basic (r1 ~= v1 ** r2 ~= pd ** pd +# offset :-> v2 ** OSZCP_Any)
-            (CMP r1, [r2+offset])
-            (r1 ~= v1 ** r2 ~= pd ** pd +# offset :-> v2 **
-             OSZCP (computeOverflow v1 v2 res) (msb res)
-                   (res == #0) carry (lsb res)).
-Proof.
-  move => E. apply TRIPLE_basic => R.
-  autounfold with eval. rewrite  /evalDstSrc/evalDstR.
-  triple_apply evalReg_rule.
-  rewrite /evalMemSpec.
-  triple_apply evalReg_rule. 
-  triple_apply triple_letGetDWORDSep. rewrite E. 
-  triple_apply triple_pre_introFlags => o s z c p. rewrite /OSZCP.
-  triple_apply triple_doSetFlagSep. 
-  triple_apply triple_doSetFlagSep. 
-  triple_apply triple_doUpdateZPS. 
-  triple_apply triple_skip. 
-Qed. 
-
-
-Lemma CMP_MR_rule (pd:BITS 32) (r1 r2:Reg) offset (v1 v2:DWORD) carry res:
-  sbbB false v2 v1 = (carry, res) ->
-  |-- basic (r1 ~= v1 ** r2 ~= pd ** pd +# offset :-> v2 ** OSZCP_Any)
-            (CMP [r2+offset], r1)
-            (r1 ~= v1 ** r2 ~= pd ** pd +# offset :-> v2 **
-             OSZCP (computeOverflow v2 v1 res) (msb res)
-                   (res == #0) carry (lsb res)).
-Proof.
-  move => E. apply TRIPLE_basic => R.
-  autounfold with eval. rewrite /evalDstSrc.
-  triple_apply evalMemSpecNone_rule. 
-  triple_apply triple_letGetDWORDSep. 
-  triple_apply evalReg_rule. rewrite E. 
-  triple_apply triple_pre_introFlags => o s z c p. rewrite /OSZCP.
-  triple_apply triple_doSetFlagSep. 
-  triple_apply triple_doSetFlagSep. 
-  triple_apply triple_doUpdateZPS.
-  triple_apply triple_skip. 
-Qed. 
-
-Lemma CMP_RR_rule (r1 r2:Reg) v1 (v2:DWORD) carry res:
-  sbbB false v1 v2 = (carry, res) ->
-  |-- basic (r1 ~= v1 ** r2 ~= v2 ** OSZCP_Any) (CMP r1, r2)
-            (r1 ~= v1 ** r2 ~= v2 **
-              OSZCP (computeOverflow v1 v2 res) (msb res)
-                    (res == #0) carry (lsb res)).
-Proof.
-  move => E. apply TRIPLE_basic => R.
-  autounfold with eval. 
-  rewrite /evalDstSrc/evalDstR.
-  triple_apply evalReg_rule. 
-  triple_apply evalReg_rule.
-  rewrite E.
-  triple_apply triple_pre_introFlags => o s z c p. rewrite /OSZCP.
-  triple_apply triple_doSetFlagSep. 
-  triple_apply triple_doSetFlagSep. 
-  triple_apply triple_doUpdateZPS. 
-  triple_apply triple_skip. 
-Qed.
 
 Lemma TEST_self_rule (r:Reg) (v:DWORD) :
   |-- basic (r ~= v ** OSZCP_Any) (TEST r, r)
